Initial renaming of theorems

src/theory/abstract_hoare_logic/abstract_hoare_logicSimps.sig
@@ -1,0 +1,6 @@
+signature abstract_hoare_logicSimps =
+sig
+   include Abbrev
+
+   val bir_wm_SS : simpLib.ssfrag
+end
