src/theory/abstract_hoare_logic/abstract_hoare_logicSimps.sml
@@ -1,0 +1,15 @@
+structure abstract_hoare_logicSimps :> abstract_hoare_logicSimps =
+struct
+
+open HolKernel boolLib liteLib simpLib Parse bossLib;
+open abstract_hoare_logicTheory;
+
+val wm_type = mk_thy_type {Tyop="abstract_model_t",
+                           Thy="abstract_hoare_logic",
+                           Args=[``:bir_state_t``,
+                                 ``:bir_label_t``]
+                          };
+
+val bir_wm_SS = rewrites (flatten (map type_rws [wm_type]));
+
+end
