src/theory/tools/comp/bir_wm_instScript.sml
@@ -67,7 +67,7 @@ val bir_etl_wm_def =
   |>`;
 
 (* bir_exec_to_labels_triple_def *)
-(* weak_triple_def *)
+(* abstract_jgmt_def *)
 
 val bir_exec_to_labels_triple_precond_def = Define `
   bir_exec_to_labels_triple_precond st pre prog =
@@ -93,10 +93,10 @@ val bir_exec_to_labels_triple_postcond_def = Define `
 `;
 
 
-(* BIR map triple, mirroring weak_map_triple *)
-val bir_map_triple_def = Define `
-  bir_map_triple prog invariant (l:bir_label_t) ls ls' pre post =
-    weak_map_triple (bir_etl_wm prog)
+(* BIR map triple, mirroring abstract_simp_jgmt *)
+val bir_simp_jgmt_def = Define `
+  bir_simp_jgmt prog invariant (l:bir_label_t) ls ls' pre post =
+    abstract_simp_jgmt (bir_etl_wm prog)
       (\s. bir_exec_to_labels_triple_precond s invariant prog)
       l ls ls'
       (\s. bir_exec_to_labels_triple_precond s pre prog)
@@ -496,17 +496,17 @@ CASE_TAC >| [
 (* BIR map triple theorems                           *)
 (*****************************************************)
 
-(* Obtaining a bir_map_triple from a bir_exec_to_labels_triple *)
-val bir_label_ht_impl_weak_ht =
-  store_thm("bir_label_ht_impl_weak_ht",
+(* Obtaining a bir_simp_jgmt from a bir_exec_to_labels_triple *)
+val bir_label_jgmt_impl_weak_jgmt =
+  store_thm("bir_label_jgmt_impl_weak_jgmt",
   ``!prog l ls pre post.
     ls <> {} ==>
     bir_exec_to_labels_triple prog l ls pre post ==>
-    bir_map_triple prog bir_exp_true l ls {} pre post``,
+    bir_simp_jgmt prog bir_exp_true l ls {} pre post``,
 
 FULL_SIMP_TAC (std_ss++bir_wm_SS)
-              [bir_map_triple_def, weak_map_triple_def,
-               weak_triple_def, bir_etl_wm_def,
+              [bir_simp_jgmt_def, abstract_simp_jgmt_def,
+               abstract_jgmt_def, bir_etl_wm_def,
                bir_exec_to_labels_triple_def,
                bir_exec_to_labels_triple_precond_def,
                bir_exec_to_labels_triple_postcond_def] >>
@@ -524,18 +524,18 @@ ASM_SIMP_TAC std_ss [bir_eval_exp_TF, bir_is_bool_exp_env_REWRS]
 );
 
 (* This theorem moves ending labels which are implicitly
- * blacklisted by the postcondition from the whitelist of a bir_map_triple to the blacklist. *)
-val bir_map_triple_move_to_blacklist = store_thm("bir_map_triple_move_to_blacklist",
+ * blacklisted by the postcondition from the whitelist of a bir_simp_jgmt to the blacklist. *)
+val bir_simp_wl_to_bl_rule_thm = store_thm("bir_simp_wl_to_bl_rule_thm",
   ``!prog inv l wlist blist pre post elabel.
-    bir_map_triple prog inv l wlist blist pre post ==>
+    bir_simp_jgmt prog inv l wlist blist pre post ==>
     elabel IN wlist ==>
     wlist DELETE elabel <> {} ==>
     (post elabel = bir_exp_false) ==>
-    bir_map_triple prog inv l (wlist DELETE elabel) (elabel INSERT blist) pre post``,
+    bir_simp_jgmt prog inv l (wlist DELETE elabel) (elabel INSERT blist) pre post``,
 
 REPEAT STRIP_TAC >>
-FULL_SIMP_TAC std_ss [bir_map_triple_def] >>
-irule weak_map_move_to_blacklist >>
+FULL_SIMP_TAC std_ss [bir_simp_jgmt_def] >>
+irule abstract_simp_wl_to_bl_rule_thm >>
 ASSUME_TAC bir_model_is_weak >>
 QSPECL_X_ASSUM ``!prog. _`` [`prog`] >>
 FULL_SIMP_TAC std_ss [] >>
@@ -544,17 +544,17 @@ SIMP_TAC std_ss [bir_exec_to_labels_triple_postcond_def] >>
 FULL_SIMP_TAC (std_ss++bir_wm_SS) [bir_etl_wm_def, bir_eval_exp_TF, bir_val_TF_dist]
 );
 
-val bir_map_triple_move_set_to_blacklist = store_thm("bir_map_triple_move_set_to_blacklist",
+val bir_simp_wl_to_bl_set_rule_thm = store_thm("bir_simp_wl_to_bl_set_rule_thm",
   ``!prog inv l wlist blist pre post elabels.
-    bir_map_triple prog inv l wlist blist pre post ==>
+    bir_simp_jgmt prog inv l wlist blist pre post ==>
     FINITE elabels ==>
     elabels PSUBSET wlist ==>
     (!elabel. elabel IN elabels ==> (post elabel = bir_exp_false)) ==>
-    bir_map_triple prog inv l (wlist DIFF elabels) (elabels UNION blist) pre post``,
+    bir_simp_jgmt prog inv l (wlist DIFF elabels) (elabels UNION blist) pre post``,
 
 REPEAT STRIP_TAC >>
-FULL_SIMP_TAC std_ss [bir_map_triple_def, pred_setTheory.UNION_COMM] >>
-irule weak_map_move_set_to_blacklist >>
+FULL_SIMP_TAC std_ss [bir_simp_jgmt_def, pred_setTheory.UNION_COMM] >>
+irule abstract_simp_wl_to_bl_set_rule_thm >>
 ASSUME_TAC bir_model_is_weak >>
 QSPECL_X_ASSUM ``!prog. _`` [`prog`] >>
 FULL_SIMP_TAC std_ss [] >>
@@ -565,19 +565,19 @@ FULL_SIMP_TAC (std_ss++bir_wm_SS) [bir_etl_wm_def, bir_eval_exp_TF, bir_val_TF_d
 );
 
 
-val bir_map_weakening_rule_thm = store_thm("bir_map_weakening_rule_thm",
+val bir_simp_post_weak_rule_thm = store_thm("bir_simp_post_weak_rule_thm",
   ``!prog invariant l ls ls' pre post1 post2.
     (!st.
      st.bst_pc.bpc_label IN ls ==>
      (bir_eval_exp (post1 st.bst_pc.bpc_label) st.bst_environ = SOME bir_val_true) ==>
      (bir_eval_exp (post2 st.bst_pc.bpc_label) st.bst_environ = SOME bir_val_true)
     ) ==>
-    bir_map_triple prog invariant l ls ls' pre post1 ==>
-    bir_map_triple prog invariant l ls ls' pre post2``,
+    bir_simp_jgmt prog invariant l ls ls' pre post1 ==>
+    bir_simp_jgmt prog invariant l ls ls' pre post2``,
 
 REPEAT STRIP_TAC >>
-FULL_SIMP_TAC std_ss [bir_map_triple_def] >>
-irule weak_map_weakening_rule_thm >>
+FULL_SIMP_TAC std_ss [bir_simp_jgmt_def] >>
+irule abstract_simp_post_weak_rule_thm >>
 REPEAT STRIP_TAC >- (
   METIS_TAC [bir_model_is_weak]
 ) >>
@@ -596,17 +596,17 @@ REPEAT STRIP_TAC >| [
 );
 
 
-val bir_taut_map_pre_str_rule_thm = store_thm("bir_taut_map_pre_str_rule_thm",
+val bir_simp_taut_pre_str_rule_thm = store_thm("bir_simp_taut_pre_str_rule_thm",
   ``!prog invariant l ls ls' pre1 pre2 post.
     ((bir_vars_of_exp pre2) SUBSET (bir_vars_of_program prog)) ==>
     ((bir_vars_of_exp pre1) SUBSET (bir_vars_of_program prog)) ==>
     bir_exp_is_taut
       (BExp_BinExp BIExp_Or (BExp_UnaryExp BIExp_Not pre2) pre1) ==>
-    bir_map_triple prog invariant l ls ls' pre1 post ==>
-    bir_map_triple prog invariant l ls ls' pre2 post``,
+    bir_simp_jgmt prog invariant l ls ls' pre1 post ==>
+    bir_simp_jgmt prog invariant l ls ls' pre2 post``,
 
 REPEAT STRIP_TAC >>
-FULL_SIMP_TAC std_ss [bir_map_triple_def, weak_map_triple_def, weak_triple_def,
+FULL_SIMP_TAC std_ss [bir_simp_jgmt_def, abstract_simp_jgmt_def, abstract_jgmt_def,
                       bir_exec_to_labels_triple_precond_def] >>
 REPEAT STRIP_TAC >>
 PAT_X_ASSUM ``!s. _`` (fn thm => ASSUME_TAC (Q.SPEC `s` thm)) >>
@@ -639,17 +639,17 @@ METIS_TAC []
 );
 
 
-val bir_taut_map_post_weak_rule_thm = store_thm("bir_taut_map_post_weak_rule_thm",
+val bir_simp_taut_post_weak_rule_thm = store_thm("bir_simp_taut_post_weak_rule_thm",
   ``!prog invariant l ls l2 ls' pre post1 post2.
     ((bir_vars_of_exp (post1 l2)) SUBSET (bir_vars_of_program prog)) ==>
     ((bir_vars_of_exp (post2 l2)) SUBSET (bir_vars_of_program prog)) ==>
     (!l'. (l' <> l2) ==> (post1 l' = post2 l')) ==>
     bir_exp_is_taut
       (BExp_BinExp BIExp_Or (BExp_UnaryExp BIExp_Not (post1 l2)) (post2 l2)) ==>
-    bir_map_triple prog invariant l ls ls' pre post1 ==>
-    bir_map_triple prog invariant l ls ls' pre post2``,
+    bir_simp_jgmt prog invariant l ls ls' pre post1 ==>
+    bir_simp_jgmt prog invariant l ls ls' pre post2``,
 
-FULL_SIMP_TAC std_ss [bir_map_triple_def, weak_map_triple_def, weak_triple_def,
+FULL_SIMP_TAC std_ss [bir_simp_jgmt_def, abstract_simp_jgmt_def, abstract_jgmt_def,
                       bir_exec_to_labels_triple_postcond_def] >>
 REPEAT STRIP_TAC >>
 PAT_X_ASSUM ``!s. _`` (fn thm => ASSUME_TAC (Q.SPEC `s` thm)) >>
@@ -682,18 +682,18 @@ METIS_TAC [bir_exp_equivTheory.bir_impl_equiv, bir_exp_tautologiesTheory.bir_exp
 );
 
 
-val bir_map_std_seq_comp_thm =
-  store_thm("bir_map_std_seq_comp_thm",
+val bir_simp_std_seq_rule_thm =
+  store_thm("bir_simp_std_seq_rule_thm",
   ``!prog ls1 ls1' ls2 ls2' invariant l pre1 post1 post2.
     ls1' SUBSET ls2 ==>
     (ls1 INTER ls1' = EMPTY) ==>
-    bir_map_triple prog invariant l ls1 ls2 pre1 post1 ==>
-    (!l1. (l1 IN ls1) ==> (bir_map_triple prog invariant l1 ls1' ls2' (post1 l1) post2)) ==>
-    bir_map_triple prog invariant l ls1' (ls2 INTER ls2') pre1 post2``,
+    bir_simp_jgmt prog invariant l ls1 ls2 pre1 post1 ==>
+    (!l1. (l1 IN ls1) ==> (bir_simp_jgmt prog invariant l1 ls1' ls2' (post1 l1) post2)) ==>
+    bir_simp_jgmt prog invariant l ls1' (ls2 INTER ls2') pre1 post2``,
 
 REPEAT STRIP_TAC >>
-FULL_SIMP_TAC std_ss [bir_map_triple_def] >>
-irule weak_map_std_seq_comp_thm >>
+FULL_SIMP_TAC std_ss [bir_simp_jgmt_def] >>
+irule abstract_simp_std_seq_rule_thm >>
 REPEAT STRIP_TAC >- (
   METIS_TAC [bir_model_is_weak]
 ) >> (
@@ -706,10 +706,10 @@ REPEAT STRIP_TAC >> (
 ) >| [
   QSPECL_X_ASSUM ``!l1. _`` [`l1`] >>
   REV_FULL_SIMP_TAC std_ss [] >>
-  FULL_SIMP_TAC std_ss [weak_map_triple_def, weak_triple_def,
+  FULL_SIMP_TAC std_ss [abstract_simp_jgmt_def, abstract_jgmt_def,
                         bir_exec_to_labels_triple_precond_def],
 
-  FULL_SIMP_TAC (std_ss++bir_wm_SS) [weak_map_triple_def,
+  FULL_SIMP_TAC (std_ss++bir_wm_SS) [abstract_simp_jgmt_def,
                                      bir_exec_to_labels_triple_precond_def,
                                      bir_exec_to_labels_triple_postcond_def,
                                      bir_etl_wm_def]
@@ -721,22 +721,22 @@ val iv2i_def = Define `
     iv2i (BVal_Imm i) = i
 `;
 
-val bir_map_signed_loop_thm = store_thm("bir_map_signed_loop_thm",
+val bir_simp_signed_loop_rule_thm = store_thm("bir_simp_signed_loop_rule_thm",
   ``!prog l wl bl invariant C1 variant post.
     (* Compute in place using proof procedures: *)
-    (*   These two needed to use weak_map_loop_thm *)
+    (*   These two needed to use abstract_simp_loop_rule_thm *)
     (type_of_bir_exp variant = SOME (BType_Imm Bit64)) ==>
     bir_vars_of_exp variant SUBSET bir_vars_of_program prog ==>
     (*   These two needed to prove bir_is_bool_exp_env ms.bst_environ C1 *)
     bir_is_bool_exp C1 ==>
     (bir_vars_of_exp C1) SUBSET (bir_vars_of_program prog) ==>
-    (* Extra for weak_map_loop_thm *)
+    (* Extra for abstract_simp_loop_rule_thm *)
     l NOTIN wl ==>
     l NOTIN bl ==>
     (wl INTER bl = {}) ==>
     (* Obtain bir_loop contract through some rule: *)
     (!x.
-     bir_map_triple prog invariant l ({l} UNION wl) bl
+     bir_simp_jgmt prog invariant l ({l} UNION wl) bl
        (BExp_BinExp BIExp_And C1
 	  (BExp_BinPred BIExp_Equal variant (BExp_Const (Imm64 x)))
        )
@@ -749,29 +749,29 @@ val bir_map_signed_loop_thm = store_thm("bir_map_signed_loop_thm",
 		    (BExp_Const (Imm64 0w)) variant))
 	    else bir_exp_false)
     ) ==>
-    bir_map_triple prog bir_exp_true l wl bl
+    bir_simp_jgmt prog bir_exp_true l wl bl
       (BExp_BinExp BIExp_And invariant (BExp_UnaryExp BIExp_Not C1)) post ==>
-    bir_map_triple prog bir_exp_true l wl bl
+    bir_simp_jgmt prog bir_exp_true l wl bl
       invariant
       post``,
 
-FULL_SIMP_TAC std_ss [bir_map_triple_def] >>
+FULL_SIMP_TAC std_ss [bir_simp_jgmt_def] >>
 REPEAT STRIP_TAC >>
 ASSUME_TAC bir_model_is_weak >>
 QSPECL_X_ASSUM ``!prog. _`` [`prog`] >>
-(* 1. Use weak_map_loop_thm *)
-Q.SUBGOAL_THEN `weak_map_triple (bir_etl_wm prog)
+(* 1. Use abstract_simp_loop_rule_thm *)
+Q.SUBGOAL_THEN `abstract_simp_jgmt (bir_etl_wm prog)
      (\s. bir_exec_to_labels_triple_precond s bir_exp_true prog) l wl bl
      (\s. bir_exec_to_labels_triple_precond s invariant prog)
      (\s'. bir_exec_to_labels_triple_postcond s' post prog) <=>
-  weak_map_triple (bir_etl_wm prog)
+  abstract_simp_jgmt (bir_etl_wm prog)
      (\s. T) l wl bl
      (\s. bir_exec_to_labels_triple_precond s invariant prog)
      (\s'. bir_exec_to_labels_triple_postcond s' post prog)`
   (fn thm => SIMP_TAC std_ss [thm]) >- (
   SIMP_TAC std_ss [bir_exec_to_labels_triple_precond_def] >>
-  FULL_SIMP_TAC std_ss [weak_map_triple_def] >>
-  SIMP_TAC std_ss [weak_triple_def] >>
+  FULL_SIMP_TAC std_ss [abstract_simp_jgmt_def] >>
+  SIMP_TAC std_ss [abstract_jgmt_def] >>
   EQ_TAC >> (
     REPEAT STRIP_TAC >>
     QSPECL_X_ASSUM ``!s. _`` [`s`] >>
@@ -780,16 +780,16 @@ Q.SUBGOAL_THEN `weak_map_triple (bir_etl_wm prog)
     FULL_SIMP_TAC std_ss [bir_exec_to_labels_triple_postcond_def]
   )
 ) >>
-irule weak_map_loop_thm >>
+irule abstract_simp_loop_rule_thm >>
 FULL_SIMP_TAC std_ss [] >>
 Q.EXISTS_TAC `\s. bir_eval_exp C1 s.bst_environ = SOME bir_val_true` >>
 Q.EXISTS_TAC `\s. b2n (iv2i (THE (bir_eval_exp variant s.bst_environ)))` >>
 STRIP_TAC >| [
   GEN_TAC >>
-  FULL_SIMP_TAC std_ss [weak_map_triple_def] >>
+  FULL_SIMP_TAC std_ss [abstract_simp_jgmt_def] >>
   (* Remove unnecessary assumption *)
-  Q.PAT_X_ASSUM `weak_triple a b c d e` (fn thm => ALL_TAC) >>
-  FULL_SIMP_TAC std_ss [weak_triple_def] >>
+  Q.PAT_X_ASSUM `abstract_jgmt a b c d e` (fn thm => ALL_TAC) >>
+  FULL_SIMP_TAC std_ss [abstract_jgmt_def] >>
   SIMP_TAC std_ss [bir_exec_to_labels_triple_precond_def] >>
   REPEAT STRIP_TAC >>
   QSPECL_X_ASSUM ``!x. _`` [`n2w x`] >>
@@ -857,7 +857,7 @@ STRIP_TAC >| [
 
   (* Remove unnecessary assumption *)
   Q.PAT_X_ASSUM `!x. _` (fn thm => ALL_TAC) >>
-  FULL_SIMP_TAC std_ss [weak_map_triple_def, weak_triple_def] >>
+  FULL_SIMP_TAC std_ss [abstract_simp_jgmt_def, abstract_jgmt_def] >>
   REPEAT STRIP_TAC >>
   QSPECL_X_ASSUM ``!s. _`` [`ms`] >>
   REV_FULL_SIMP_TAC std_ss [bir_exec_to_labels_triple_precond_def, GSYM bir_and_equiv] >>
@@ -874,22 +874,22 @@ STRIP_TAC >| [
 );
 
 
-val bir_map_unsigned_loop_thm = store_thm("bir_map_unsigned_loop_thm",
+val bir_simp_unsigned_loop_rule_thm = store_thm("bir_simp_unsigned_loop_rule_thm",
   ``!prog l wl bl invariant C1 variant post.
     (* Compute in place using proof procedures: *)
-    (*   These two needed to use weak_map_loop_thm *)
+    (*   These two needed to use abstract_simp_loop_rule_thm *)
     (type_of_bir_exp variant = SOME (BType_Imm Bit64)) ==>
     bir_vars_of_exp variant SUBSET bir_vars_of_program prog ==>
     (*   These two needed to prove bir_is_bool_exp_env ms.bst_environ C1 *)
     bir_is_bool_exp C1 ==>
     (bir_vars_of_exp C1) SUBSET (bir_vars_of_program prog) ==>
-    (* Extra for weak_map_loop_thm *)
+    (* Extra for abstract_simp_loop_rule_thm *)
     l NOTIN wl ==>
     l NOTIN bl ==>
     (wl INTER bl = {}) ==>
     (* Obtain bir_loop contract through some rule: *)
     (!x.
-     bir_map_triple prog invariant l ({l} UNION wl) bl
+     bir_simp_jgmt prog invariant l ({l} UNION wl) bl
        (BExp_BinExp BIExp_And C1
 	  (BExp_BinPred BIExp_Equal variant (BExp_Const (Imm64 x)))
        )
@@ -902,30 +902,30 @@ val bir_map_unsigned_loop_thm = store_thm("bir_map_unsigned_loop_thm",
 		    (BExp_Const (Imm64 0w)) variant))
 	    else bir_exp_false)
     ) ==>
-    bir_map_triple prog bir_exp_true l wl bl
+    bir_simp_jgmt prog bir_exp_true l wl bl
       (BExp_BinExp BIExp_And invariant (BExp_UnaryExp BIExp_Not C1)) post ==>
-    bir_map_triple prog bir_exp_true l wl bl
+    bir_simp_jgmt prog bir_exp_true l wl bl
       invariant
       post``,
 
 
-FULL_SIMP_TAC std_ss [bir_map_triple_def] >>
+FULL_SIMP_TAC std_ss [bir_simp_jgmt_def] >>
 REPEAT STRIP_TAC >>
 ASSUME_TAC bir_model_is_weak >>
 QSPECL_X_ASSUM ``!prog. _`` [`prog`] >>
-(* 1. Use weak_map_loop_thm *)
-Q.SUBGOAL_THEN `weak_map_triple (bir_etl_wm prog)
+(* 1. Use abstract_simp_loop_rule_thm *)
+Q.SUBGOAL_THEN `abstract_simp_jgmt (bir_etl_wm prog)
      (\s. bir_exec_to_labels_triple_precond s bir_exp_true prog) l wl bl
      (\s. bir_exec_to_labels_triple_precond s invariant prog)
      (\s'. bir_exec_to_labels_triple_postcond s' post prog) <=>
-  weak_map_triple (bir_etl_wm prog)
+  abstract_simp_jgmt (bir_etl_wm prog)
      (\s. T) l wl bl
      (\s. bir_exec_to_labels_triple_precond s invariant prog)
      (\s'. bir_exec_to_labels_triple_postcond s' post prog)`
   (fn thm => SIMP_TAC std_ss [thm]) >- (
   SIMP_TAC std_ss [bir_exec_to_labels_triple_precond_def] >>
-  FULL_SIMP_TAC std_ss [weak_map_triple_def] >>
-  SIMP_TAC std_ss [weak_triple_def] >>
+  FULL_SIMP_TAC std_ss [abstract_simp_jgmt_def] >>
+  SIMP_TAC std_ss [abstract_jgmt_def] >>
   EQ_TAC >> (
     REPEAT STRIP_TAC >>
     QSPECL_X_ASSUM ``!s. _`` [`s`] >>
@@ -934,16 +934,16 @@ Q.SUBGOAL_THEN `weak_map_triple (bir_etl_wm prog)
     FULL_SIMP_TAC std_ss [bir_exec_to_labels_triple_postcond_def]
   )
 ) >>
-irule weak_map_loop_thm >>
+irule abstract_simp_loop_rule_thm >>
 FULL_SIMP_TAC std_ss [] >>
 Q.EXISTS_TAC `\s. bir_eval_exp C1 s.bst_environ = SOME bir_val_true` >>
 Q.EXISTS_TAC `\s. b2n (iv2i (THE (bir_eval_exp variant s.bst_environ)))` >>
 STRIP_TAC >| [
   GEN_TAC >>
-  FULL_SIMP_TAC std_ss [weak_map_triple_def] >>
+  FULL_SIMP_TAC std_ss [abstract_simp_jgmt_def] >>
   (* Remove unnecessary assumption *)
-  Q.PAT_X_ASSUM `weak_triple a b c d e` (fn thm => ALL_TAC) >>
-  FULL_SIMP_TAC std_ss [weak_triple_def] >>
+  Q.PAT_X_ASSUM `abstract_jgmt a b c d e` (fn thm => ALL_TAC) >>
+  FULL_SIMP_TAC std_ss [abstract_jgmt_def] >>
   SIMP_TAC std_ss [bir_exec_to_labels_triple_precond_def] >>
   REPEAT STRIP_TAC >>
   QSPECL_X_ASSUM ``!x. _`` [`n2w x`] >>
@@ -1009,7 +1009,7 @@ STRIP_TAC >| [
 
   (* Remove unnecessary assumption *)
   Q.PAT_X_ASSUM `!x. _` (fn thm => ALL_TAC) >>
-  FULL_SIMP_TAC std_ss [weak_map_triple_def, weak_triple_def] >>
+  FULL_SIMP_TAC std_ss [abstract_simp_jgmt_def, abstract_jgmt_def] >>
   REPEAT STRIP_TAC >>
   QSPECL_X_ASSUM ``!s. _`` [`ms`] >>
   REV_FULL_SIMP_TAC std_ss [bir_exec_to_labels_triple_precond_def, GSYM bir_and_equiv] >>
@@ -1027,19 +1027,19 @@ STRIP_TAC >| [
 
 (* Shrinking the whitelist is possible if the corresponding
  * postcondition never holds. *)
-val bir_map_subset_rule_thm =
- store_thm("bir_map_subset_rule_thm",
+val bir_simp_wl_subset_rule_thm =
+ store_thm("bir_simp_wl_subset_rule_thm",
   ``!prog l ls1 ls2 pre post.
     ls1 <> {} ==>
     (!st. (bir_eval_exp (post st.bst_pc.bpc_label) st.bst_environ = SOME bir_val_true) ==>
           (~(st.bst_pc.bpc_label IN ls2))
     ) ==>
-    bir_map_triple prog bir_exp_true l (ls1 UNION ls2) {} pre post ==>
-    bir_map_triple prog bir_exp_true l ls1 {} pre post``,
+    bir_simp_jgmt prog bir_exp_true l (ls1 UNION ls2) {} pre post ==>
+    bir_simp_jgmt prog bir_exp_true l ls1 {} pre post``,
 
 REPEAT STRIP_TAC >>
-REV_FULL_SIMP_TAC std_ss [bir_map_triple_def, weak_map_triple_def,
-                          weak_triple_def] >>
+REV_FULL_SIMP_TAC std_ss [bir_simp_jgmt_def, abstract_simp_jgmt_def,
+                          abstract_jgmt_def] >>
 REPEAT STRIP_TAC >> (
   FULL_SIMP_TAC (std_ss++pred_setLib.PRED_SET_ss) []
 ) >> (
@@ -1056,17 +1056,18 @@ REPEAT STRIP_TAC >> (
 )
 );
 
-val bir_map_subset_blacklist_rule_thm =
-  store_thm("bir_map_subset_blacklist_rule_thm",
+val bir_simp_bl_subset_rule_thm =
+  store_thm("bir_simp_bl_subset_rule_thm",
   ``!prog invariant l wl bl bl' pre post.
     bl' SUBSET bl ==>
-    bir_map_triple prog invariant l wl bl pre post ==>
-    bir_map_triple prog invariant l wl bl' pre post``,
+    bir_simp_jgmt prog invariant l wl bl pre post ==>
+    bir_simp_jgmt prog invariant l wl bl' pre post``,
 
-METIS_TAC [bir_map_triple_def, bir_model_is_weak,
-           weak_map_subset_blacklist_rule_thm]
+METIS_TAC [bir_simp_jgmt_def, bir_model_is_weak,
+           abstract_simp_bl_subset_rule_thm]
 );
 
+(* TODO: Move this? *)
 val bir_exec_to_labels_triple_precond_subprogram =
   store_thm("bir_exec_to_labels_triple_precond_subprogram",
   ``!prog1 prog2 s pre.
@@ -1078,6 +1079,7 @@ METIS_TAC [bir_exec_to_labels_triple_precond_def,
            bir_env_vars_are_initialised_SUBPROGRAM]
 );
 
+(* TODO: Move this? *)
 val bir_is_valid_pc_exec =
   store_thm("bir_is_valid_pc_exec",
   ``!s pre prog ls l' n n0 s'.
@@ -1122,17 +1124,17 @@ Cases_on `bir_get_current_statement prog s.bst_pc` >- (
 FULL_SIMP_TAC std_ss [GSYM bir_get_current_statement_IS_SOME]
 );
 
-val bir_map_prog_comp_thm =
-  store_thm("bir_map_prog_comp_thm",
+val bir_simp_prog_comp_rule_thm =
+  store_thm("bir_simp_prog_comp_rule_thm",
   ``!prog1 prog2 invariant wl bl l pre post.
     bir_is_subprogram prog1 prog2 ==>
     bir_is_valid_labels prog2 ==>
-    bir_map_triple prog1 invariant l wl bl pre post ==>
-    bir_map_triple prog2 invariant l wl bl pre post``,
+    bir_simp_jgmt prog1 invariant l wl bl pre post ==>
+    bir_simp_jgmt prog2 invariant l wl bl pre post``,
 
 REPEAT STRIP_TAC >>
-FULL_SIMP_TAC std_ss [bir_map_triple_def, weak_map_triple_def] >>
-FULL_SIMP_TAC (std_ss++bir_wm_SS) [weak_triple_def,
+FULL_SIMP_TAC std_ss [bir_simp_jgmt_def, abstract_simp_jgmt_def] >>
+FULL_SIMP_TAC (std_ss++bir_wm_SS) [abstract_jgmt_def,
 				   bir_etl_wm_def, bir_weak_trs_def] >>
 REPEAT STRIP_TAC >>
 QSPECL_X_ASSUM ``!s. _`` [`s`] >>
@@ -1164,18 +1166,18 @@ CONJ_TAC >> (
 )
 );
 
-(* Sketch for alternative proof using weak_map_model_comp_rule_thm
+(* Sketch for alternative proof using abstract_simp_model_comp_rule_thm
 val bir_map_prog_comp_alt_thm =
   store_thm("bir_map_prog_comp_alt_thm",
   ``!prog1 prog2 invariant wl bl l pre post.
     bir_is_subprogram prog1 prog2 ==>
     bir_is_valid_labels prog2 ==>
-    bir_map_triple prog1 invariant l wl bl pre post ==>
-    bir_map_triple prog2 invariant l wl bl pre post``,
+    bir_simp_jgmt prog1 invariant l wl bl pre post ==>
+    bir_simp_jgmt prog2 invariant l wl bl pre post``,
 
 REPEAT STRIP_TAC >>
-FULL_SIMP_TAC std_ss [bir_map_triple_def] >>
-irule weak_map_model_comp_rule_thm >>
+FULL_SIMP_TAC std_ss [bir_simp_jgmt_def] >>
+irule abstract_simp_model_comp_rule_thm >>
 FULL_SIMP_TAC std_ss [bir_model_is_weak] >>
 Q.EXISTS_TAC `bir_etl_wm prog1` >>
 REPEAT STRIP_TAC >| [
@@ -1183,7 +1185,7 @@ REPEAT STRIP_TAC >| [
   FULL_SIMP_TAC (std_ss++bir_wm_SS) [bir_etl_wm_def],
 
   (* (bir_etl_wm prog2).weak ms ls ms' *)
-  FULL_SIMP_TAC (std_ss++bir_wm_SS) [bir_etl_wm_def, bir_weak_trs_def, weak_map_triple_def] >>
+  FULL_SIMP_TAC (std_ss++bir_wm_SS) [bir_etl_wm_def, bir_weak_trs_def, abstract_simp_jgmt_def] >>
   Cases_on `bir_exec_to_labels ls prog2 ms` >> Cases_on `bir_exec_to_labels ls prog1 ms` >> (
     FULL_SIMP_TAC (std_ss++holBACore_ss) []
   ) >> (
@@ -1205,8 +1207,8 @@ REPEAT STRIP_TAC >| [
 
   FULL_SIMP_TAC std_ss [bir_model_is_weak],
 
-  FULL_SIMP_TAC std_ss [weak_map_triple_def] >>
-  FULL_SIMP_TAC (std_ss++bir_wm_SS) [weak_triple_def,
+  FULL_SIMP_TAC std_ss [abstract_simp_jgmt_def] >>
+  FULL_SIMP_TAC (std_ss++bir_wm_SS) [abstract_jgmt_def,
 				     bir_etl_wm_def, bir_weak_trs_def] >>
   REPEAT STRIP_TAC >>
   IMP_RES_TAC bir_exec_to_labels_triple_precond_subprogram >>
