src/theory/abstract_hoare_logic/abstract_hoare_logicScript.sml
@@ -1,0 +1,447 @@
+open HolKernel Parse boolLib bossLib;
+
+open bir_auxiliaryLib;
+
+open bir_auxiliaryTheory;
+
+val _ = new_theory "abstract_hoare_logic";
+
+(* Transition system *)
+val _ = Datatype `abstract_model_t =
+  <|(* Transition function *)
+    trs : 'a -> 'a option;
+    (* Weak transition relation *)
+    weak : 'a -> ('b -> bool) -> 'a -> bool;
+    (* A function to obtain the control state from a state.
+     * This allows for isolating parts of the state that
+     * the weak transition is provably oblivious to. *)
+    pc : 'a -> 'b
+   |>`;
+
+(* An abstract model is a weak model, if this property is fulfilled.
+ * This is how the weak transition is forced to be related to
+ * the single transition.  *)
+val weak_model_def = Define `
+  weak_model m =
+    !ms ls ms'.
+      (m.weak ms ls ms') =
+        ?n.
+          ((n > 0) /\
+           (FUNPOW_OPT m.trs n ms = SOME ms') /\
+           ((m.pc ms') IN ls)
+          ) /\
+          !n'.
+            (((n' < n) /\ (n' > 0)) ==>
+            ?ms''.
+              (FUNPOW_OPT m.trs n' ms = SOME ms'') /\
+              (~((m.pc ms'') IN ls))
+            )`;
+
+
+val weak_comp_thm = prove(``
+  !m.
+  weak_model m ==>
+  !ms ls1 ls2 ms' ms''.
+  (m.weak ms (ls1 UNION ls2) ms') ==> (~((m.pc ms') IN ls2)) ==>
+  (m.weak ms' ls2 ms'') ==> (m.weak ms ls2 ms'')``,
+
+REPEAT STRIP_TAC >>
+REV_FULL_SIMP_TAC std_ss [weak_model_def] >>
+EXISTS_TAC ``n'+n:num`` >>
+ASSUME_TAC (Q.SPECL [`m.trs`, `n'`, `n`, `ms`, `ms'`, `ms''`] FUNPOW_OPT_ADD_thm) >>
+REV_FULL_SIMP_TAC arith_ss [] >>
+REPEAT STRIP_TAC >>
+Cases_on `n'' < n'` >- (
+  METIS_TAC [pred_setTheory.IN_UNION]
+) >>
+Cases_on `n'' = n'` >- (
+  METIS_TAC []
+) >>
+SUBGOAL_THEN ``n'':num = (n''-n')+n'`` ASSUME_TAC >- (FULL_SIMP_TAC arith_ss []) >>
+QSPECL_X_ASSUM ``!n''.((n'' < n:num) /\ (n'' > 0)) ==> P`` [`n''-n':num`] >>
+REV_FULL_SIMP_TAC arith_ss [] >>
+ASSUME_TAC (Q.SPECL [`m.trs`, `n'`, `n''-n'`, `ms`, `ms'`, `ms'''`] FUNPOW_OPT_ADD_thm) >>
+REV_FULL_SIMP_TAC arith_ss []
+);
+
+
+val weak_unique_thm = prove(``
+  !m.
+  (weak_model m) ==>
+  !ms ls ms' ms''.
+  (m.weak ms ls ms') ==>
+  (m.weak ms ls ms'') ==>
+  (ms' = ms'')
+``,
+
+REPEAT STRIP_TAC >>
+REV_FULL_SIMP_TAC std_ss [weak_model_def] >>
+Q.SUBGOAL_THEN `n = n'` (FULLSIMP_BY_THM arith_ss)  >>
+Cases_on `n < n'` >- (
+   QSPECL_X_ASSUM ``!n'':num.(n'' < n' /\ n'' > 0) ==> P`` [`n:num`] >>
+   REV_FULL_SIMP_TAC std_ss [] 
+) >>
+Cases_on `n > n'` >- (
+   QSPECL_X_ASSUM ``!n'':num.(n'' < n /\ n'' > 0) ==> P`` [`n':num`] >>
+   REV_FULL_SIMP_TAC arith_ss [] 
+) >>
+FULL_SIMP_TAC arith_ss [] 
+);
+
+val weak_union_thm = prove(``
+  !m.
+  weak_model m ==>
+  !ms ls1 ls2 ms'.
+  (m.weak ms (ls1 UNION ls2) ms') ==>
+  (~ ((m.pc ms') IN ls1)) ==>
+  (m.weak ms ls2 ms')``,
+
+REPEAT STRIP_TAC >>
+REV_FULL_SIMP_TAC std_ss [weak_model_def] >>
+Q.EXISTS_TAC `n` >>
+METIS_TAC [pred_setTheory.IN_UNION]
+);
+
+val weak_union2_thm = prove(``
+  !m.
+  weak_model m ==>
+  !ms ls1 ls2 ms'.
+  (m.weak ms (ls1 UNION ls2) ms') ==>
+  (((m.pc ms') IN ls2)) ==>
+  (m.weak ms ls2 ms')``,
+
+REPEAT STRIP_TAC >>
+REV_FULL_SIMP_TAC std_ss [weak_model_def] >>
+Q.EXISTS_TAC `n` >>
+METIS_TAC [pred_setTheory.IN_UNION]
+);
+
+val weak_union_singleton_thm = prove(``
+  !m.
+  weak_model m ==>
+  !ms l1 ls2 ms'.
+  (m.weak ms ({l1} UNION ls2) ms') ==>
+  ((m.pc ms') <> l1) ==>
+  (m.weak ms ls2 ms')``,
+
+METIS_TAC [weak_union_thm, pred_setTheory.IN_SING]
+);
+
+val weak_singleton_pc_thm = prove(``
+  !m.
+  weak_model m ==>
+  !ms e ms'.
+  (m.weak ms {e} ms') ==> ((m.pc ms') = e)``,
+
+METIS_TAC [weak_model_def, pred_setTheory.IN_SING]
+);
+
+
+val weak_pc_in_thm = prove(``
+  !m.
+  weak_model m ==>
+  !ms ls ms'.
+  (m.weak ms ls ms') ==> ((m.pc ms') IN ls)``,
+
+METIS_TAC [weak_model_def]
+);
+
+val weak_union_pc_not_in_thm = store_thm("weak_union_pc_not_in_thm",
+  ``!m.
+    weak_model m ==>
+    !ms e ls1 ls2 ms'.
+    (m.weak ms (ls1 UNION ls2) ms') ==>
+    (~((m.pc ms') IN ls2)) ==>
+    (m.weak ms ls1 ms')``,
+
+REPEAT STRIP_TAC >>
+REV_FULL_SIMP_TAC std_ss [weak_model_def] >>
+METIS_TAC [pred_setTheory.IN_UNION]
+);
+
+
+
+(* Judgment of the logic *)
+(* Pre and post usually have conditions on execution mode and code in memory,
+   also post is usually a map that depends on the end state address *)
+val abstract_jgmt_def = Define `
+  abstract_jgmt m (l:'a) (ls:'a->bool) pre post =
+  !ms .
+   ((m.pc ms) = l) ==> (pre ms) ==>
+   ?ms'. ((m.weak ms ls ms') /\
+    (post ms'))
+`;
+
+
+val abstract_weak_model_comp_rule_thm = store_thm("abstract_weak_model_comp_rule_thm",
+  ``!m n l ls pre post.
+    weak_model m ==>
+    weak_model n ==>
+    (!ms ls ms'. m.weak ms ls ms' ==> n.weak ms ls ms') ==>
+    (!ms l. (n.pc ms = l)  ==> (m.pc ms = l)) ==>
+    abstract_jgmt m l ls pre post ==>
+    abstract_jgmt n l ls pre post``,
+
+REPEAT STRIP_TAC >>
+FULL_SIMP_TAC std_ss [abstract_jgmt_def] >>
+REPEAT STRIP_TAC >>
+QSPECL_X_ASSUM ``!ms. _`` [`ms`] >>
+QSPECL_X_ASSUM ``!ms. _`` [`ms`] >>
+REV_FULL_SIMP_TAC std_ss [] >>
+FULL_SIMP_TAC std_ss [] >>
+QSPECL_X_ASSUM ``!ms ls ms'. _`` [`ms`, `ls`, `ms'`] >>
+REV_FULL_SIMP_TAC std_ss [] >>
+Q.EXISTS_TAC `ms'` >>
+FULL_SIMP_TAC std_ss []
+);
+
+
+val abstract_case_rule_thm = prove(``
+!m l ls pre post C1.
+  abstract_jgmt m l ls (\ms. (pre ms) /\ (C1 ms)) post ==>
+  abstract_jgmt m l ls (\ms. (pre ms) /\ (~(C1 ms))) post ==>
+  abstract_jgmt m l ls pre post
+``,
+
+REPEAT STRIP_TAC >>
+FULL_SIMP_TAC std_ss [abstract_jgmt_def] >>
+METIS_TAC []
+);
+
+val abstract_conseq_rule_thm =
+  store_thm("abstract_conseq_rule_thm",
+  ``!m. 
+    !l ls pre1 pre2 post1 post2.
+    weak_model m ==>
+    (!ms. ((m.pc ms) = l) ==> (pre2 ms) ==> (pre1 ms)) ==>
+    (!ms. ((m.pc ms) IN ls) ==> (post1 ms) ==> (post2 ms)) ==>
+    abstract_jgmt m l ls pre1 post1 ==>
+    abstract_jgmt m l ls pre2 post2
+  ``,
+
+SIMP_TAC std_ss [abstract_jgmt_def] >>
+REPEAT STRIP_TAC >>
+METIS_TAC [weak_pc_in_thm]
+);
+
+
+
+val abstract_subset_rule_thm =
+ store_thm("abstract_subset_rule_thm",
+  ``!m.  ! l ls1 ls2 pre post .
+    weak_model m ==>
+    (!ms. ((post ms) ==> (~((m.pc ms) IN ls2)))) ==>
+    abstract_jgmt m l (ls1 UNION ls2) pre post ==>
+    abstract_jgmt m l ls1 pre post``,
+
+REPEAT STRIP_TAC >>
+REV_FULL_SIMP_TAC std_ss [abstract_jgmt_def] >>
+REPEAT STRIP_TAC >>
+QSPECL_X_ASSUM ``!x. _`` [`ms`] >>
+METIS_TAC [weak_union_pc_not_in_thm]
+);
+
+
+val abstract_seq_rule_thm = store_thm("abstract_seq_rule_thm",
+  ``!m l ls1 ls2 pre post.
+    weak_model m ==>
+    abstract_jgmt m l (ls1 UNION ls2) pre post ==>
+    (!l1. (l1 IN ls1) ==>
+    (abstract_jgmt m l1 ls2 post post)) ==>
+    abstract_jgmt m l ls2 pre post``,
+
+REPEAT STRIP_TAC >>
+SIMP_TAC std_ss [abstract_jgmt_def] >>
+REPEAT STRIP_TAC >>
+PAT_X_ASSUM ``(abstract_jgmt m l (ls1 UNION ls2) pre  post)``
+              (fn thm => ASSUME_TAC (SIMP_RULE std_ss [abstract_jgmt_def] thm)) >>
+QSPECL_X_ASSUM ``!x.P`` [`ms`] >>
+REV_FULL_SIMP_TAC std_ss [] >>
+Cases_on `(m.pc ms') IN ls2` >- (
+  METIS_TAC [weak_union2_thm]
+) >>
+Q.SUBGOAL_THEN `(m.pc ms') IN ls1` ASSUME_TAC >- (
+  METIS_TAC [weak_union_thm, weak_pc_in_thm]
+) >>
+QSPECL_X_ASSUM  ``!l1. _`` [`m.pc ms'`] >>
+REV_FULL_SIMP_TAC std_ss [abstract_jgmt_def] >>
+QSPECL_X_ASSUM  ``!m. _`` [`ms'`] >>
+REV_FULL_SIMP_TAC std_ss[] >>
+ASSUME_TAC (Q.SPECL [`m`] weak_comp_thm) >>
+METIS_TAC []
+);
+
+
+val abstract_conj_rule_thm = prove(``
+  !m.
+  weak_model m ==>
+  !l ls pre post1 post2.
+  abstract_jgmt m l ls pre post1 ==>
+  abstract_jgmt m l ls pre post2 ==>
+  abstract_jgmt m l ls pre (\ms. (post1 ms) /\ (post2 ms))``,
+
+REPEAT STRIP_TAC >>
+FULL_SIMP_TAC std_ss [abstract_jgmt_def] >>
+REPEAT STRIP_TAC >>
+METIS_TAC [weak_unique_thm]
+);
+
+
+
+val loop_step_def = Define `
+  loop_step m ms var l le invariant C1 =
+    let x:num = var ms in
+    (\ms'. (m.weak ms ({l} UNION le) ms') /\
+	   ((invariant ms) /\ (C1 ms)) /\
+	   (((m.pc ms')=l) /\ (invariant ms') /\ ((var ms') < x) /\ ((var ms') >= 0))
+    )
+`;
+
+val loop_fun_defn =
+  Hol_defn "loop_fun" `
+    loop_fun m ms var l le invariant C1  =
+      let MS' = loop_step m ms var l le invariant C1 in
+      if MS' = {} then ms
+      else let ms' = (CHOICE MS') in
+	(loop_fun m ms' var l le invariant C1)
+`;
+
+(*
+Defn.tgoal loop_fun_defn
+*)
+val (loop_fun_eqns, loop_fun_ind) = Defn.tprove(loop_fun_defn,
+  FULL_SIMP_TAC std_ss [loop_step_def] >>
+  WF_REL_TAC `measure (\(m, ms,var,l,le,invariant,C1). var ms)` >>
+  REPEAT STRIP_TAC >>
+  REV_FULL_SIMP_TAC std_ss [LET_DEF] >>
+  Q.ABBREV_TAC `MS' =  (\ms'.
+               m.weak ms ({l} UNION le) ms' /\ (invariant ms /\ C1 ms) /\
+               ((m.pc ms') = l) /\ invariant ms' /\ var ms' < var ms)` >>
+  ASSUME_TAC (ISPEC ``MS':'a->bool`` pred_setTheory.CHOICE_DEF)  >>
+  REV_FULL_SIMP_TAC std_ss [] >>
+  FULL_SIMP_TAC std_ss [Abbr `MS'`, pred_setTheory.IN_ABS]
+);
+
+
+val abstract_loop_jgmt_def = Define `
+  abstract_loop_jgmt m l le invariant C1 var =
+    ((~(l IN le)) /\
+    (!x. (abstract_jgmt m l ({l} UNION le) (\ms. (invariant ms) /\ (C1 ms) /\ ((var ms) = x:num))
+         (\ms.(((m.pc ms)=l) /\ (invariant ms) /\ ((var ms) < x) /\ ((var ms) >= 0))))))
+`;
+
+val inductive_invariant_goal =
+(fst o dest_imp o concl ) (
+  Q.SPEC `(\m ms var l le invariant C1.
+	   weak_model m ==>
+	   abstract_loop_jgmt m l le invariant C1 var ==>
+	   abstract_jgmt m l le (\ms. (invariant ms) /\ (~(C1 ms))) post ==>
+	   ((invariant ms) /\ ((m.pc ms) = l) /\ (C1 ms)) ==>
+	   (?ms'. ((m.weak ms le ms') /\ (post ms'))))`
+  loop_fun_ind
+);
+
+
+val inductive_invariant = prove(``
+^inductive_invariant_goal
+``,
+
+REPEAT STRIP_TAC >>
+FULL_SIMP_TAC std_ss [] >>
+REPEAT STRIP_TAC >>
+(* We first prove that one iteration works *)
+SUBGOAL_THEN ``(loop_step m ms var l le invariant C1) <> {}`` ASSUME_TAC  >- (
+  SIMP_TAC std_ss [loop_step_def, LET_DEF] >>
+  FULL_SIMP_TAC std_ss [abstract_loop_jgmt_def] >>
+  QSPECL_X_ASSUM ``!x. _`` [`(var (ms)):num`] >>
+  FULL_SIMP_TAC std_ss [abstract_jgmt_def] >>
+  QSPECL_X_ASSUM ``!x. _`` [`ms`] >>
+  REV_FULL_SIMP_TAC std_ss [] >>
+  FULL_SIMP_TAC std_ss [GSYM pred_setTheory.MEMBER_NOT_EMPTY] >>
+  EXISTS_TAC ``ms'':'a`` >>
+  FULL_SIMP_TAC std_ss [pred_setTheory.SPECIFICATION]
+) >>
+FULL_SIMP_TAC std_ss [] >>
+
+Q.ABBREV_TAC `MS' = (loop_step m ms var l le invariant C1)` >>
+Q.ABBREV_TAC `ms' = CHOICE MS'` >>
+
+(* We prove that the invariant is preserved *)
+SUBGOAL_THEN ``(loop_step m ms var l le invariant C1) ms'`` ASSUME_TAC >- (
+  FULL_SIMP_TAC std_ss [Abbr `ms'`] >>
+  ASSUME_TAC (ISPEC ``MS':'a->bool`` pred_setTheory.CHOICE_DEF) >>
+  REV_FULL_SIMP_TAC std_ss [pred_setTheory.SPECIFICATION]
+) >>
+Q.SUBGOAL_THEN `invariant ms'` ASSUME_TAC >- (
+  FULL_SIMP_TAC std_ss [ loop_step_def, LET_DEF]
+) >>
+FULL_SIMP_TAC std_ss [] >>
+Q.SUBGOAL_THEN `(m.pc ms') = l` ASSUME_TAC >- (
+  FULL_SIMP_TAC std_ss [ loop_step_def, LET_DEF]
+) >>
+FULL_SIMP_TAC std_ss [] >>
+
+(* If we exit the loop *)
+Cases_on `~ (C1 ms')` >- (
+  (FULL_SIMP_TAC std_ss [loop_step_def, LET_DEF]) >>
+  (FULL_SIMP_TAC std_ss [abstract_jgmt_def]) >>
+  QSPECL_X_ASSUM  ``!x. _`` [`ms'`] >>
+  (REV_FULL_SIMP_TAC std_ss []) >>
+  ASSUME_TAC (Q.SPECL [`m`] weak_comp_thm) >>
+  REV_FULL_SIMP_TAC std_ss [] >>
+  QSPECL_X_ASSUM ``!x. _`` [`ms`, `{l}`, `le`, `ms'`, `ms''`] >>
+  REV_FULL_SIMP_TAC (std_ss) [SINGLETONS_UNION_thm] >>
+  Q.SUBGOAL_THEN `l NOTIN le` (FULLSIMP_BY_THM std_ss) >- (
+    FULL_SIMP_TAC std_ss [abstract_loop_jgmt_def, pred_setTheory.IN_SING]
+  ) >>
+  METIS_TAC []
+) >> (
+  FULL_SIMP_TAC std_ss []
+) >> (
+  FULL_SIMP_TAC std_ss [loop_step_def, LET_DEF]
+) >>
+ASSUME_TAC (Q.SPECL [`m`] weak_comp_thm) >>
+REV_FULL_SIMP_TAC std_ss [] >>
+QSPECL_X_ASSUM ``!x. _`` [`ms`, `{l}`, `le`, `ms'`, `ms''`] >>
+REV_FULL_SIMP_TAC (std_ss) [SINGLETONS_UNION_thm] >>
+  Q.SUBGOAL_THEN `l NOTIN le` (FULLSIMP_BY_THM std_ss) >- (
+    FULL_SIMP_TAC std_ss [abstract_loop_jgmt_def, pred_setTheory.IN_SING]
+  ) >>
+  METIS_TAC []
+);
+
+
+
+
+val abstract_loop_rule_tmp_thm = 
+MP 
+(Q.SPEC `(\m ms var l le invariant C1.
+weak_model m ==>
+abstract_loop_jgmt m l le invariant C1 var ==>
+abstract_jgmt m l le (\ms. (invariant ms) /\ (~(C1 ms))) post ==>
+((invariant ms) /\ ((m.pc ms) = l) /\ (C1 ms)) ==>
+ (?ms'. ((m.weak ms le ms') /\ (post ms'))))` loop_fun_ind) inductive_invariant;
+
+val abstract_loop_rule_thm = store_thm("abstract_loop_rule_thm",
+  ``!m.
+    weak_model m ==>
+    !l le invariant C1 var post.
+    abstract_loop_jgmt m l le invariant C1 var ==>
+    abstract_jgmt m l le (\ms. (invariant ms) /\ (~(C1 ms))) post ==>
+    abstract_jgmt m l le invariant post``,
+
+REPEAT STRIP_TAC >>
+SIMP_TAC std_ss [abstract_jgmt_def] >>
+REPEAT STRIP_TAC >>
+ASSUME_TAC (Q.SPECL [`m`, `ms`, `var`, `l`, `le`, `invariant`, `C1`] abstract_loop_rule_tmp_thm) >>
+FULL_SIMP_TAC std_ss [] >>
+REV_FULL_SIMP_TAC std_ss [] >>
+Cases_on `C1 ms` >- (
+  FULL_SIMP_TAC std_ss [] >>
+  Q.EXISTS_TAC `ms'`>>
+  FULL_SIMP_TAC std_ss []
+) >>
+FULL_SIMP_TAC std_ss [abstract_jgmt_def] 
+);
+
+val _ = export_theory();
